investigations/bedrock2/RiscvMachineWithCavaDevice/MMIOToCava.v
@@ -1,9 +1,16 @@
 Require Import Coq.ZArith.ZArith.
 Require Import Coq.Lists.List. Import ListNotations.
-Require Import coqutil.Word.Interface coqutil.Map.Interface.
+Require Import Coq.Logic.FunctionalExtensionality.
+Require Import Coq.Logic.PropExtensionality.
+Require Import Coq.micromega.Lia.
+Require Import coqutil.Tactics.Tactics.
+Require Import coqutil.Word.Interface coqutil.Word.Properties coqutil.Map.Interface.
 Require Import coqutil.Map.OfListWord.
 Require Import coqutil.Datatypes.PropSet.
+Require Import coqutil.Tactics.Simp.
+Require Import bedrock2.ZnWords.
 Require Import Bedrock2Experiments.StateMachineSemantics.
+Require Import Bedrock2Experiments.StateMachineProperties.
 Require Import riscv.Platform.MetricRiscvMachine.
 Require Import riscv.Utility.FreeMonad.
 Require Import riscv.Utility.runsToNonDet.
@@ -12,6 +19,39 @@ Require Import Bedrock2Experiments.RiscvMachineWithCavaDevice.InternalMMIOMachin
 Require Import Bedrock2Experiments.RiscvMachineWithCavaDevice.DetIncrMachine.
 Require Import Bedrock2Experiments.StateMachineMMIOSpec.
 
+Class device_implements_state_machine{word: word.word 32}{mem: map.map word Byte.byte}
+      (D: device)(sp: StateMachineSemantics.parameters.parameters 32 word mem) :=
+{
+  mmioAddrs_match: sameset StateMachineSemantics.parameters.isMMIOAddr device.isMMIOAddr;
+
+  device_state_related: StateMachineSemantics.parameters.state -> D -> Prop;
+
+  initial_state_is_reset_state: forall sH,
+      parameters.is_initial_state sH <-> device_state_related sH device.reset_state;
+
+  (* each device state is mapped to at most one state machine state *)
+  state_machine_state_unique: forall sL sH1 sH2,
+      device_state_related sH1 sL ->
+      device_state_related sH2 sL ->
+      sH1 = sH2;
+
+  state_machine_read_to_device_read: forall n r v sH sH' sL,
+      parameters.read_step n sH r v sH' ->
+      device_state_related sH sL ->
+      exists sL',
+        device.runUntilResp true false (word_to_bv (parameters.reg_addr r)) (word_to_bv (word.of_Z 0))
+                            device.maxRespDelay sL = (Some (word_to_bv v), sL') /\
+        device_state_related sH' sL';
+
+  state_machine_write_to_device_write: forall n r v sH sH' sL,
+      parameters.write_step n sH r v sH' ->
+      device_state_related sH sL ->
+      exists sL' ignored,
+        device.runUntilResp false true (word_to_bv (parameters.reg_addr r)) (word_to_bv v)
+                            device.maxRespDelay sL = (Some ignored, sL') /\
+        device_state_related sH' sL';
+}.
+
 Section WithParams.
   Context {word : Interface.word.word 32} {word_ok: word.ok word}
           {Registers: map.map Z word} {Registers_ok: map.ok Registers}
@@ -19,22 +59,22 @@ Section WithParams.
           {state_machine_params: StateMachineSemantics.parameters.parameters 32 word mem}
           {state_machine_params_ok: StateMachineSemantics.parameters.ok state_machine_params}
           {D: device}
-          (device_state_related: StateMachineSemantics.parameters.state -> D -> Prop).
+          {DI: device_implements_state_machine D state_machine_params}.
 
-  Inductive related(t0: list LogItem): MetricRiscvMachine -> ExtraRiscvMachine D -> Prop :=
+  Inductive related: MetricRiscvMachine -> ExtraRiscvMachine D -> Prop :=
     mkRelated: forall regs pc npc m xAddrs (t: list LogItem) mc s d,
       execution t s ->
       device_state_related s d ->
       map.undef_on m StateMachineSemantics.parameters.isMMIOAddr ->
       disjoint (of_list xAddrs) StateMachineSemantics.parameters.isMMIOAddr ->
-      related t0
+      related
         {| MetricRiscvMachine.getMachine :=
              {| getRegs := regs;
                 getPc := pc;
                 getNextPc := npc;
                 getMem := m;
                 getXAddrs := xAddrs;
-                getLog := t ++ t0; |};
+                getLog := t; |};
            getMetrics := mc; |}
         {| ExtraRiscvMachine.getMachine :=
              {| getRegs := regs;
@@ -42,7 +82,7 @@ Section WithParams.
                 getNextPc := npc;
                 getMem := m;
                 getXAddrs := xAddrs;
-                getLog := t0; |};
+                getLog := []; |};
            getExtraState := d |}.
 
   Definition stepH(initialL: MetricRiscvMachine)(post: MetricRiscvMachine -> Prop): Prop :=
@@ -51,46 +91,423 @@ Section WithParams.
 
   Variable sched: schedule.
 
-  Lemma stateMachine_to_cava_1: forall t0 (initialH: MetricRiscvMachine) (initialL: ExtraRiscvMachine D)
+  Lemma read_step_isMMIOAddrB: forall n s r v s',
+      parameters.read_step n s r v s' ->
+      device.isMMIOAddrB (parameters.reg_addr r) n = true.
+  Proof.
+    intros.
+    pose proof (parameters.read_step_size_valid _ _ _ _ _ H) as V. simpl in V.
+    pose proof (parameters.read_step_isMMIOAddr _ _ _ _ _ H) as P.
+    unfold device.isMMIOAddrB.
+    eapply andb_true_intro.
+    rewrite !Z.leb_le.
+    replace parameters.isMMIOAddr with device.isMMIOAddr in P. 2: {
+      symmetry. extensionality x. apply propositional_extensionality. unfold iff.
+      pose proof mmioAddrs_match as Q. unfold sameset, subset, elem_of in Q. destruct Q. eauto.
+    }
+    unfold device.isMMIOAddr in P.
+    split.
+    - eapply P. lia.
+    - enough (word.unsigned (parameters.reg_addr r) + Z.of_nat n - 1 < device.addr_range_pastend).
+      1: lia.
+      pose proof (parameters.read_step_is_aligned _ _ _ _ _ H) as A.
+      specialize (P (word.add (parameters.reg_addr r) (word.of_Z (Z.of_nat n - 1)))).
+      ZnWords.
+  Qed.
+
+  Lemma write_step_isMMIOAddrB: forall n s r v s',
+      parameters.write_step n s r v s' ->
+      device.isMMIOAddrB (parameters.reg_addr r) n = true.
+  Proof.
+    intros.
+    pose proof (parameters.write_step_size_valid _ _ _ _ _ H) as V. simpl in V.
+    pose proof (parameters.write_step_isMMIOAddr _ _ _ _ _ H) as P.
+    unfold device.isMMIOAddrB.
+    eapply andb_true_intro.
+    rewrite !Z.leb_le.
+    replace parameters.isMMIOAddr with device.isMMIOAddr in P. 2: {
+      symmetry. extensionality x. apply propositional_extensionality. unfold iff.
+      pose proof mmioAddrs_match as Q. unfold sameset, subset, elem_of in Q. destruct Q. eauto.
+    }
+    unfold device.isMMIOAddr in P.
+    split.
+    - eapply P. lia.
+    - enough (word.unsigned (parameters.reg_addr r) + Z.of_nat n - 1 < device.addr_range_pastend).
+      1: lia.
+      pose proof (parameters.write_step_is_aligned _ _ _ _ _ H) as A.
+      specialize (P (word.add (parameters.reg_addr r) (word.of_Z (Z.of_nat n - 1)))).
+      ZnWords.
+  Qed.
+
+  (* Uniqueness lemmas follow from device_implements_state_machine, because they say that
+     the state machine is behaves like a deterministic Cava device.
+     Using this assumption, we can prove uniqueness once and for all, instead of individually
+     for each state machine. *)
+
+  Lemma write_step_unique: forall sz prevH prevL r v s s',
+      device_state_related prevH prevL ->
+      parameters.write_step sz prevH r v s ->
+      parameters.write_step sz prevH r v s' ->
+      s = s'.
+  Proof.
+    intros.
+    eapply state_machine_write_to_device_write in H0. 2: eassumption.
+    eapply state_machine_write_to_device_write in H1. 2: eassumption.
+    simp.
+    rewrite H0p0 in H1p0. inversion H1p0. subst. clear H1p0.
+    eapply state_machine_state_unique; eassumption.
+  Qed.
+
+  (* note: could be made stronger by also showing that the read values are equal,
+     but we don't need this here *)
+  Lemma read_step_unique: forall sz prevH prevL r v s s',
+      device_state_related prevH prevL ->
+      parameters.read_step sz prevH r v s ->
+      parameters.read_step sz prevH r v s' ->
+      s = s'.
+  Proof.
+    intros.
+    eapply state_machine_read_to_device_read in H0. 2: eassumption.
+    eapply state_machine_read_to_device_read in H1. 2: eassumption.
+    simp.
+    rewrite H0p0 in H1p0. inversion H1p0. subst. clear H1p0.
+    eapply state_machine_state_unique; eassumption.
+  Qed.
+
+  Lemma step_unique: forall a prevH prevL args rets s s',
+      device_state_related prevH prevL ->
+      step a prevH args rets s ->
+      step a prevH args rets s' ->
+      s = s'.
+  Proof.
+    unfold step. intros.
+    destruct (String.prefix MMIOLabels.WRITE_PREFIX a).
+    - simp.
+      replace sz0 with sz in *. 2: {
+        pose proof (parameters.write_step_size_valid _ _ _ _ _ H0p3) as V1. simpl in V1.
+        pose proof (parameters.write_step_size_valid _ _ _ _ _ H1p1) as V2. simpl in V2.
+        destruct V1 as [? | [? | [? | ?]]]; destruct V2 as [? | [? | [? | ?]]]; subst;
+          reflexivity || discriminate || contradiction.
+      }
+      eapply parameters.reg_addr_unique in H0p0. subst r1.
+      eapply write_step_unique; eassumption.
+    - destruct (String.prefix MMIOLabels.READ_PREFIX a). 2: contradiction. simp.
+      replace sz0 with sz in *. 2: {
+        pose proof (parameters.read_step_size_valid _ _ _ _ _ H0p3) as V1. simpl in V1.
+        pose proof (parameters.read_step_size_valid _ _ _ _ _ H1p1) as V2. simpl in V2.
+        destruct V1 as [? | [? | [? | ?]]]; destruct V2 as [? | [? | [? | ?]]]; subst;
+          reflexivity || discriminate || contradiction.
+      }
+      eapply parameters.reg_addr_unique in H0p0. subst r0.
+      eapply read_step_unique; eassumption.
+  Qed.
+
+  Lemma execution_exists_related: forall t sH,
+      execution t sH -> exists sL, device_state_related sH sL.
+  Proof.
+    induction t; cbn; intros.
+    - exists device.reset_state. eapply initial_state_is_reset_state. assumption.
+    - destruct a as (((mGive & a) & args) & (mReceive & rets)). simp.
+      specialize (IHt _ Hp0). destruct IHt as (prevL & IH).
+      unfold step in Hp1.
+      destruct (String.prefix MMIOLabels.WRITE_PREFIX a).
+      + simp. eapply state_machine_write_to_device_write in Hp1p1. 2: eassumption.
+        simp. eauto.
+      + simp. eapply state_machine_read_to_device_read in Hp1p1. 2: eassumption.
+        simp. eauto.
+  Qed.
+
+  Lemma execution_unique: forall t s s',
+      execution t s -> execution t s' -> s = s'.
+  Proof.
+    induction t; cbn [execution]; intros.
+    - eapply state_machine_state_unique.
+      + eapply initial_state_is_reset_state. exact H.
+      + eapply initial_state_is_reset_state. exact H0.
+    - destruct a as (((mGive & a) & args) & (mReceive & rets)).
+      destruct H as (prev & E & St). destruct H0 as (prev' & E' & St').
+      specialize (IHt _ _ E E'). subst prev'.
+      eapply execution_exists_related in E. simp.
+      eapply step_unique; eassumption.
+  Qed.
+
+  Lemma bv_to_word_word_to_bv: forall v, bv_to_word (word_to_bv v) = v.
+  Proof.
+    intros. unfold bv_to_word, word_to_bv.
+  Admitted.
+
+  Lemma execution_read_cons: forall n r (v: HList.tuple Byte.byte n) t s1 s2,
+      execution t s1 ->
+      parameters.read_step n s1 r (word.of_Z (LittleEndian.combine n v)) s2 ->
+      execution (MinimalMMIO.mmioLoadEvent (W := mkWords) (parameters.reg_addr r) v :: t) s2.
+  Proof. intros. eapply execution_step_read; eauto. Qed.
+
+  Lemma execution_write_cons: forall n r (v: HList.tuple Byte.byte n) t s1 s2,
+      execution t s1 ->
+      parameters.write_step n s1 r (word.of_Z (LittleEndian.combine n v)) s2 ->
+      execution (MinimalMMIO.mmioStoreEvent (W := mkWords) (parameters.reg_addr r) v :: t) s2.
+  Proof. intros. eapply execution_step_write; eauto. Qed.
+
+  Lemma preserve_undef_on_unchecked: forall sz (m: mem) a v1 v2 s,
+      Memory.load_bytes sz m a = Some v1 ->
+      map.undef_on m s ->
+      map.undef_on (Memory.unchecked_store_bytes sz m a v2) s.
+  Proof.
+    intros.
+    refine (MinimalMMIO.preserve_undef_on _ _ _ _ _ _ _ H0).
+    unfold Memory.store_bytes.
+    match goal with
+    | |- match ?x with _ => _ end = _ => replace x with (Some v1)
+    end.
+    1: reflexivity.
+    symmetry. exact H.
+  Qed.
+
+  Lemma preserve_disjoint_of_invalidateXAddrs: forall sz xAddrs a s,
+      disjoint (of_list xAddrs) s ->
+      disjoint (of_list (Primitives.invalidateWrittenXAddrs sz a xAddrs)) s.
+  Proof.
+    induction sz; intros; cbn.
+    - assumption.
+    - change removeXAddr with (@List.removeb word word.eqb _).
+      rewrite ?ListSet.of_list_removeb.
+      eauto 10 using disjoint_diff_l.
+  Qed.
+
+  Lemma stateMachine_primitive_to_cava: forall (initialH: MetricRiscvMachine) (p: riscv_primitive)
+      (metricsUpdater: MetricLogging.MetricLog -> MetricLogging.MetricLog)
+      (postH: primitive_result p -> MetricRiscvMachine -> Prop),
+      (forall v finalH, postH v finalH -> exists s, execution finalH.(getLog) s) ->
+      MetricMinimalMMIO.interp_action (metricsUpdater, p) initialH postH ->
+      forall (initialL: ExtraRiscvMachine D),
+        related initialH initialL ->
+        exists finalH res finalL,
+          InternalMMIOMachine.interpret_action p initialL = (Some res, finalL) /\
+          postH res finalH /\
+          related finalH finalL.
+  Proof.
+    intros. inversion H1. clear H1. subst.
+    destruct p;
+      cbn -[HList.tuple Memory.load_bytes Primitives.invalidateWrittenXAddrs] in *; try contradiction.
+
+    (* GetRegister *)
+    { destruct (Z.eq_dec z 0). 1: eauto 10 using mkRelated.
+      cbn. destruct (map.get regs z); eauto 10 using mkRelated. }
+
+    (* SetRegister *)
+    { destruct (Z.eq_dec z 0). 1: eauto 10 using mkRelated.
+      unfold Monads.OStateOperations.put. cbn. eauto 10 using mkRelated. }
+
+    (* Load* *)
+    1-4: unfold MinimalMMIO.load, MinimalMMIO.nonmem_load in H0;
+      destruct H0 as [HX HL]; cbn -[HList.tuple Memory.load_bytes] in *.
+    1-4: match type of HL with
+         | match ?x with _ => _ end => destruct x eqn: E; [destruct s0|]
+         end;
+         try specialize (HX eq_refl);
+         rewrite ?(isXAddr4B_true _ _ HX);
+         eauto 10 using mkRelated.
+    1-4: simp; erewrite ?read_step_isMMIOAddrB by eassumption.
+    1-4: match goal with
+         | E1: execution _ _, E2: execution _ _ |- _ =>
+           pose proof (execution_unique _ _ _ E1 E2); subst; clear E2
+         end.
+    1-4: edestruct state_machine_read_to_device_read as (d' & RU & Rel'); [eassumption..|].
+    1-4: cbn -[HList.tuple]; rewrite RU; cbn -[HList.tuple].
+    4: { (* 64-bit MMIO is not supported: *)
+      eapply parameters.read_step_size_valid in HLp2p2. simpl in HLp2p2. exfalso. intuition congruence.
+    }
+    1-3: rewrite bv_to_word_word_to_bv;
+         rewrite word.unsigned_of_Z_nowrap by (pose proof (LittleEndian.combine_bound v); lia);
+         rewrite LittleEndian.split_combine.
+    1-3: eauto 15 using mkRelated, execution_read_cons.
+
+    (* Store* *)
+    1-4: unfold MinimalMMIO.store, MinimalMMIO.nonmem_store, Memory.store_bytes in *;
+      cbn -[HList.tuple Memory.load_bytes Memory.unchecked_store_bytes
+            Primitives.invalidateWrittenXAddrs] in *.
+    1-4: match type of H0 with
+         | match match ?x with _ => _ end with _ => _ end => destruct x eqn: E
+         end.
+    1-8: unfold Monads.OStateOperations.put;
+         cbn -[HList.tuple Memory.load_bytes Memory.unchecked_store_bytes
+               Primitives.invalidateWrittenXAddrs] in *;
+         eauto 15 using mkRelated, preserve_undef_on_unchecked, preserve_disjoint_of_invalidateXAddrs.
+    1-4: simp.
+    1-4: specialize (H _ _ H0p2); cbn in H; simp.
+    1-4: rename Hp1p2 into WS; pose proof WS as WS';
+         eapply parameters.write_step_size_valid in WS';
+         simpl in WS'; destruct WS' as [? | [? | [? | ?]]];
+         try contradiction; subst sz; try discriminate. (* <- also gets rid of 8-byte MMIO case *)
+    1-3: simp; erewrite write_step_isMMIOAddrB by eassumption.
+    1-3: match goal with
+         | E1: execution _ _, E2: execution _ _ |- _ =>
+           pose proof (execution_unique _ _ _ E1 E2); subst; clear E2
+         end.
+    1-3: edestruct state_machine_write_to_device_write as (d' & ignored & RU & Rel'); [eassumption..|].
+    1-3: cbn -[HList.tuple Primitives.invalidateWrittenXAddrs]; rewrite RU;
+         cbn -[HList.tuple Primitives.invalidateWrittenXAddrs].
+    1-3: eauto 15 using mkRelated, execution_write_cons, preserve_disjoint_of_invalidateXAddrs.
+
+    (* GetPC *)
+    { eauto 10 using mkRelated. }
+
+    (* SetPC *)
+    { unfold Monads.OStateOperations.put. eauto 10 using mkRelated. }
+
+    (* EndCycleNormal *)
+    { unfold Monads.OStateOperations.put. eauto 10 using mkRelated. }
+  Qed.
+
+  Fixpoint discard_metrics{A: Type}(p: free MetricMinimalMMIO.action MetricMinimalMMIO.result A)
+    : free riscv_primitive primitive_result A :=
+    match p with
+    | free.act (u, a) k => free.act a (fun r => discard_metrics (k r))
+    | free.ret v => free.ret v
+    end.
+
+  Lemma stateMachine_free_to_cava{A: Type}: forall (postH: A -> MetricRiscvMachine -> Prop),
+      (forall v finalH, postH v finalH -> exists s, execution finalH.(getLog) s) ->
+      forall (p: free MetricMinimalMMIO.action MetricMinimalMMIO.result A)
+             (initialH: MetricRiscvMachine),
+      free.interp MetricMinimalMMIO.interp_action p initialH postH ->
+      forall (initialL: ExtraRiscvMachine D),
+        related initialH initialL ->
+        exists finalH res finalL,
+          free.interp_as_OState InternalMMIOMachine.interpret_action (discard_metrics p) initialL =
+            (Some res, finalL) /\
+          postH res finalH /\
+          related finalH finalL.
+  Proof.
+    induction p; intros.
+    - destruct a as [u a].
+      simpl in H1.
+  Abort.
+
+  Lemma free_act_eq_inv1: forall {action : Type} {result : action -> Type} {T : Type} (a1 a2 : action)
+            (k1 : result a1 -> free action result T) (k2 : result a2 -> free action result T),
+      free.act a1 k1 = free.act a2 k2 ->
+      a1 = a2.
+  Proof. intros. inversion H. reflexivity. Qed.
+
+  Lemma free_act_eq_inv2: forall {action : Type} {result : action -> Type} {T : Type} (a : action)
+            (k1 k2 : result a -> free action result T),
+      free.act a k1 = free.act a k2 ->
+      k1 = k2.
+  Proof.
+    intros. inversion H. eapply Eqdep.EqdepTheory.inj_pair2 in H1. exact H1.
+  Qed.
+  (* Note: depends on Axiom Eqdep.Eq_rect_eq.eq_rect_eq *)
+
+  (* TODO maybe it would be better to require read_step/write_step in mmioLoad/mmioStore
+     methods of the MinimalMMIO machine, so that we would not need this lemma *)
+  Lemma invert_interp_bind_execution{A: Type}: forall (initialH: MetricRiscvMachine) u a f
+                                                      (postH: A -> MetricRiscvMachine -> Prop),
+      (forall v finalH, postH v finalH ->
+                        exists s, execution (p := state_machine_params) finalH.(getLog) s) ->
+      free.interp MetricMinimalMMIO.interp_action (free.act (u, a) f) initialH postH ->
+      exists midH,
+        MetricMinimalMMIO.interp_action (u, a) initialH midH /\
+        forall r m, midH r m -> free.interp MetricMinimalMMIO.interp_action (f r) m postH.
+  Proof.
+    intros. remember (free.act (u, a) f) as m.
+    revert dependent u. revert dependent a. revert dependent initialH.
+    induction m; intros.
+    - pose proof (free_act_eq_inv1 _ _ _ _ Heqm). subst a.
+      eapply free_act_eq_inv2 in Heqm. subst f0.
+      simpl in H1.
+      destruct a0; cbn in H1.
+      {
+        match type of H1 with
+        | _ _ ?x _ _ => remember x as m
+        end.
+        destruct m. 2: {
+          simpl in H1.
+  Abort.
+
+  Lemma stateMachine_free_to_cava{A: Type}:
+    forall (p: free MetricMinimalMMIO.action MetricMinimalMMIO.result A) (initialH: MetricRiscvMachine)
+      (postH: A -> MetricRiscvMachine -> Prop),
+      (forall v finalH, postH v finalH -> exists s, execution finalH.(getLog) s) ->
+      free.interp MetricMinimalMMIO.interp_action p initialH postH ->
+      forall (initialL: ExtraRiscvMachine D),
+        related initialH initialL ->
+        exists finalH res finalL,
+          free.interp_as_OState InternalMMIOMachine.interpret_action (discard_metrics p) initialL =
+            (Some res, finalL) /\
+          postH res finalH /\
+          related finalH finalL.
+  Proof.
+    induction p; intros.
+    - destruct a as [u a].
+      simpl in H1.
+
+      (* stuck: can't make
+         (forall v finalH, postH v finalH -> exists s, execution finalH.(getLog) s)
+         hold for intermeditate postconditions *)
+  Admitted.
+
+  Lemma stateMachine_to_cava_1: forall (initialH: MetricRiscvMachine) (initialL: ExtraRiscvMachine D)
                                        steps_done post,
-      related t0 initialH initialL ->
+      related initialH initialL ->
       stepH initialH post ->
+      (forall finalH, post finalH -> exists s, execution finalH.(getLog) s) ->
       exists finalL finalH, nth_step sched steps_done initialL = (Some tt, finalL) /\
-                            related t0 finalH finalL /\
+                            related finalH finalL /\
                             post finalH.
   Proof.
     intros.
     unfold stepH in H0.
     unfold nth_step.
-    (*
-      above the line:
-      Run.run1 with Bedrock2Experiments.Riscv.MetricMinimalMMIO.IsRiscvMachine
-      below the line:
-      Run.run1 with Bedrock2Experiments.RiscvMachineWithCavaDevice.InternalMMIOMachine.IsRiscvMachine
+    unfold Run.run1 in *.
+    unfold Monads.Bind, Monads.OState_Monad, free.Monad_free in *.
+    simpl free.bind in *.
+    cbn [free.interp free.interp_fix free.interp_body] in *.
+    eapply stateMachine_primitive_to_cava in H0.
+  Abort.
 
-      would like to say "forall monadic programs, L behaves like H" --> L needs to go through
-      monad materialization as well *)
-
-    (* not sure if useful: *)
-    pose proof (run1_sane Decode.RV32I) as A.
-    unfold MetricPrimitives.mcomp_sane, Primitives.mcomp_sat, Primitives.valid_machine,
-        MetricMinimalMMIO.MetricMinimalMMIOPrimitivesParams, MinimalMMIO.isMMIOAddr,
-        StateMachineMMIOSpec in A.
-    specialize A with (2 := H0). cbv beta in A.
-    inversion H. subst. clear H.
-    destruct A as (A & _). 1: split; assumption.
-    destruct A as (_ & finalH & Pf & Un & Dj).
+  Lemma stateMachine_to_cava_1: forall (initialH: MetricRiscvMachine) (initialL: ExtraRiscvMachine D)
+                                       steps_done post,
+      related initialH initialL ->
+      stepH initialH post ->
+      (forall finalH, post finalH -> exists s, execution finalH.(getLog) s) ->
+      exists finalL finalH, nth_step sched steps_done initialL = (Some tt, finalL) /\
+                            related finalH finalL /\
+                            post finalH.
+  Proof.
+    intros.
+    unfold stepH in H0.
+    unfold nth_step.
+    let R1 := match goal with
+              | H: context[?R1] |- _ =>
+                lazymatch R1 with
+                | Run.run1 _ => R1
+                end
+              end in
+    let R2 := match goal with
+              | |- context[?R2] =>
+                lazymatch R2 with
+                | Run.run1 _ => R2
+                end
+              end in
+    assert (R2 = discard_metrics R1). {
+      simpl.
+      f_equal.
+      extensionality x.
+      f_equal.
+      extensionality y.
 
   Admitted.
 
-  Lemma stateMachine_to_cava: forall t_initial
-                                     (initialH: MetricRiscvMachine) (initialL: ExtraRiscvMachine D)
+  Axiom TODO: False.
+
+  Lemma stateMachine_to_cava: forall (initialH: MetricRiscvMachine) (initialL: ExtraRiscvMachine D)
                                      steps_done post,
-      related t_initial initialH initialL ->
+      related initialH initialL ->
       runsTo stepH initialH post ->
       exists steps_remaining finalL finalH,
         run_rec sched steps_done steps_remaining initialL = (Some tt, finalL) /\
-        related t_initial finalH finalL /\
+        related finalH finalL /\
         post finalH.
   Proof.
     intros. revert initialL steps_done H. induction H0; intros.
@@ -98,6 +515,7 @@ Section WithParams.
     - pose proof stateMachine_to_cava_1 as One.
       specialize One with (1 := H2) (2 := H). specialize (One steps_done).
       destruct One as (midL & midH & One & Rmid & M).
+      1: case TODO.
       specialize H1 with (1 := M) (2 := Rmid). specialize (H1 (S steps_done)).
       destruct H1 as (steps_remaining & finalL & finalH & Star & Rfinal & Pfinal).
       exists (S steps_remaining). simpl. rewrite One. eauto.
